Interop: More auxiliary lemmas and proof for down_up_identity

src/test/interop/Interop.fst
@@ -338,15 +338,13 @@ let up_mem heap ptr1 addr1 ptr2 addr2 length1 length2 mem =
 let hs_equal (h0:HS.mem) (h1:HS.mem) = FStar.HyperStack.ST.equal_domains h0 h1 /\ HS.modifies Set.empty h0 h1
 
 let shift_equal_seq (b:B.buffer UInt8.t) (h0 h1: HS.mem) : Lemma
-  (requires (forall i. 0 <= i /\ i < B.length b ==> Seq.index (B.sel h0 b) (B.idx b + i) == Seq.index (B.sel h1 b) (B.idx b + i)))
+  (requires (forall i. 0 <= i /\ i < B.length b ==> Seq.index (B.as_seq h0 b) i == Seq.index (B.as_seq h1 b) i))
   (ensures (forall i. B.idx b <= i /\ i < B.idx b + B.length b ==> Seq.index (B.sel h0 b) i == Seq.index (B.sel h1 b) i)) =
   let s0 = B.sel h0 b in
   let s1 = B.sel h1 b in
   assert (forall i. 0 <= i /\ i < B.length b ==> Seq.index s0 (B.idx b + i) == Seq.index s1 (B.idx b + i));
-  assert (forall i. B.idx b <= i /\ i < B.idx b + B.length b ==> Seq.index s0 (B.idx b + (i - B.idx b)) == Seq.index s1 (B.idx b + (i - B.idx b)));
-  assert (forall i. {:pattern (Seq.index s1 i)} B.idx b <= i /\ i < B.idx b + B.length b ==> Seq.index s1 i == Seq.index s1 (B.idx b + (i - B.idx b)));
-  assert (forall i. {:pattern (Seq.index s0 i)} B.idx b <= i /\ i < B.idx b + B.length b ==> Seq.index s0 (B.idx b + (i - B.idx b)) == Seq.index s0 i);
- ()
+  assert (forall i. i == i - B.idx b + B.idx b);
+  ()
 
 let non_seq_as_seq_equal (b:B.buffer UInt8.t) (h0 h1: HS.mem) : Lemma 
   (requires (B.as_seq h0 b == B.as_seq h1 b /\ equal_non_seq_buf h0 h1 b))
@@ -354,11 +352,25 @@ let non_seq_as_seq_equal (b:B.buffer UInt8.t) (h0 h1: HS.mem) : Lemma
  let s0 = B.sel h0 b in
  let s1 = B.sel h1 b in
  assert (forall i. 0 <= i /\ i < B.idx b ==> Seq.index s0 i == Seq.index s1 i);
- assert (forall i. 0 <= i /\ i < B.length b ==> Seq.index (B.as_seq h0 b) i == Seq.index (B.as_seq h1 b) i);
- assert (forall i. 0 <= i /\ i < B.length b ==> Seq.index s0 (B.idx b + i) == Seq.index s1 (B.idx b + i));
  shift_equal_seq b h0 h1;
  assert (forall i. B.idx b <= i /\ i < B.idx b + B.length b ==> Seq.index s0 i == Seq.index s1 i);
  ()
+
+let same_seq_equal (b1:B.buffer UInt8.t) (b2:B.buffer UInt8.t{B.max_length b1 = B.max_length b2}) (h0 h1:HS.mem) : Lemma
+  (requires (B.as_ref b1 == B.as_ref b2 /\ B.frameOf b1 = B.frameOf b2 /\ B.as_seq h0 b1 == B.as_seq h1 b1 /\ B.as_seq h0 b2 == B.as_seq h1 b2 /\ (forall i. 0 <= i /\ i < B.max_length b1 /\ i < B.max_length b2 ==>
+      not (i >= B.idx b1 && i < B.idx b1 + B.length b1) ==>
+      not (i >= B.idx b2 && i < B.idx b2 + B.length b2) ==>
+      Seq.index (B.sel h0 b1) i == Seq.index (B.sel h1 b1) i /\
+      Seq.index (B.sel h0 b2) i == Seq.index (B.sel h1 b2) i)))
+  (ensures (Seq.equal (B.sel h0 b1) (B.sel h1 b1)) /\ Seq.equal (B.sel h0 b1) (B.sel h1 b1)) =
+  let s1_0 = B.sel h0 b1 in
+  let s1_1 = B.sel h1 b1 in
+  let s2_0 = B.sel h0 b2 in
+  let s2_1 = B.sel h1 b2 in
+  assert (s1_0 == s2_0);
+  shift_equal_seq b1 h0 h1;
+  shift_equal_seq b2 h0 h1;
+  ()
   
 val down_up_identity: (mem:HS.mem) -> (ptr1:(B.buffer UInt8.t){B.live mem ptr1})  -> (ptr2:(B.buffer UInt8.t){B.live mem ptr2 /\ B.disjoint ptr1 ptr2})
   -> (length1:nat{length1 = B.length ptr1}) -> (length2:nat{length2 = B.length ptr2}) -> Lemma 
@@ -378,7 +390,7 @@ let down_up_identity mem ptr1 ptr2 length1 length2 =
   let m_inter = Map.restrict (HS.mod_set s) mem.HS.h in
   let m2 = Map.concat new_mem.HS.h m_inter in
    // We only have to focus on the heap for this rid
-  assert (forall r'. r' <> r ==> Map.sel m1 r' == Map.sel m2 r');
+   assert (forall r'. r' <> r ==> Map.sel m1 r' == Map.sel m2 r');
   let h0 = Map.sel m1 r in // Heap
   let h1 = Map.sel m2 r in // Heap
   let ref = B.as_ref ptr1 in
@@ -386,20 +398,26 @@ let down_up_identity mem ptr1 ptr2 length1 length2 =
   equal_heap h0 h1;
   assert (Heap.equal_dom h0 h1);
   assert (HS.modifies_ref r (Set.singleton addrof) mem new_mem);
-  assert (Heap.modifies (Set.singleton addrof) (Map.sel mem.HS.h r) (Map.sel new_mem.HS.h r));
+  assert (Heap.modifies (Set.singleton addrof) (Map.sel mem.HS.h r) (Map.sel new_mem.HS.h r)); // Only this address is modified in this heap
   assert (Seq.equal (B.as_seq mem ptr1) (B.as_seq new_mem ptr1));
   assert (B.as_seq mem ptr1 == B.as_seq new_mem ptr1);
+  assert (Seq.equal (B.as_seq mem ptr2) (B.as_seq new_mem ptr2));
+  assert (B.as_seq mem ptr2 == B.as_seq new_mem ptr2);
   if (B.as_addr ptr1 <> B.as_addr ptr2 || B.frameOf ptr1 <> B.frameOf ptr2) then begin
     non_seq_as_seq_equal ptr1 mem new_mem;
-    assert (Seq.equal (B.sel mem ptr1) (B.sel new_mem ptr1));
-    admit()
+    assert (Seq.equal (B.sel mem ptr1) (B.sel new_mem ptr1))
   end
-  else admit()
-  //assert (B.sel mem ptr1 == B.sel new_mem ptr1);
-  
+  else begin
+    ref_extensionality h0 (B.as_ref ptr1) (B.as_ref ptr2);
+    same_seq_equal ptr1 ptr2 mem new_mem;
+    assert (Seq.equal (B.sel mem ptr1) (B.sel new_mem ptr1))
+  end;
+  assert (B.sel mem ptr1 == B.sel new_mem ptr1); // The complete underlying sequence (not just B.as_seq) is the same before and after
+  assert (Heap.sel h1 ref == B.sel new_mem ptr1);
+
   // assume (h1 == Heap.upd h0 ref (B.sel new_mem ptr1));
   // assert (Heap.sel h0 ref == Heap.sel h1 ref);
-  // admit()
+  admit()
 
  // assert (forall (a:Type) (rel:Preorder.preorder a) (r:Heap.mref a rel). Heap.addr_of r == addrof /\ Heap.is_mm r == Heap.is_mm (B.as_ref ptr1) ==> Heap.sel h0 r == Heap.sel h1 r);
 //  assume (forall (a:Type) (rel:Preorder.preorder a) (r:Heap.mref a rel). Heap.addr_of r == addrof ==> Heap.sel h0 r == Heap.sel h1 r);
